\documentclass[12pt]{article}

\title{Assignment 2023-08-22}
\author{Robert Krency}
\date{}

\usepackage{subfiles}

\usepackage{tikz}
%Tikz Library
\usetikzlibrary{angles, quotes, intersections}



\usepackage{pgfplots}
\usepgfplotslibrary{polar}

%Notation
\usepackage{physics}
\usepackage{bm}

%AMS
\usepackage{amsmath}
\usepackage{amsfonts}
\usepackage{amssymb}
\usepackage{amsthm}

%Stuff
\usepackage{graphicx}
\usepackage{tabularx}
\usepackage{multicol}
\usepackage{algpseudocode}
\usepackage{algorithm}
\usepackage{enumitem}

\usepackage{setspace}
\onehalfspacing

% Geometry 
\usepackage{geometry}
\geometry{letterpaper, left=1in, top=1in, right=1in, bottom=1in}

\setlength\columnsep{20pt}

% Fancy Header
\usepackage{fancyhdr, lastpage}
\fancypagestyle{plain}{
  \fancyhf{}    % Clear header/footer
  \fancyhead[L]{ Math 3440 - Differential Equations}
  \fancyhead[R]{RDK - F23}
  \fancyfoot[C]{Page \thepage\ of \pageref{LastPage}}
}
\pagestyle{plain}

% Add vertical spacing to tables
\renewcommand{\arraystretch}{1.8}

% Macros
\newcommand{\definition}[1]{\underline{\textbf{#1}}}

\newenvironment{rcases}
  {\left.\begin{aligned}}
  {\end{aligned}\right\rbrace}

% Begin Document
\begin{document}

\maketitle

\section*{Section 1}

\begin{enumerate}
  \item Confirm the claimed solution in example 1.1.5 is actually a solution to the differential equation.

  ODE: \(y' + 3y = 2\) \\ 
  General Solution: \(y = \frac{2}{3} + Ce^{-3t}\)

  \begin{proof}
    \begin{align*}
      y' = & -3Ce^{-3t} \\
      y' + 3y = & -3Ce^{-3t} + 3(\frac{2}{3} + Ce^{-3t}) \\
      = & -3Ce^{-3t} + frac{6}{3} + 3Ce^{-3t} \\
      = & \ 2.
    \end{align*}
  \end{proof}
  
  \item Show the following are solutions to the indicated differential equations.
  
  \begin{enumerate}
    \item \(y = e^{-x}\) is a solution to \(y' + y = 0\)
    \begin{proof}
      \begin{align*}
        y' = & -e^{-x} \\
        y' + y = & -e^{-x} + e^{-x} = 0.
      \end{align*}  
    \end{proof}

    \pagebreak
    \item \(y = x^2\) is a solution to \(xy' = 2y\)
    \begin{proof}
      \begin{align*}
        y' = & \ 2x \\
        xy' = & \ x * 2x = 2x^2 = 2y.
      \end{align*}
    \end{proof}
    
    \item \(y = \sqrt{1 + x^2}\) is a solution to \((1 + x^2)y' = xy\)
    \begin{proof}
      \begin{align*}
        y' = &\  \frac{1}{2} {(1 + x^2)}^{-\frac{1}{2}} * 2x \\
        = & \ x {(1 + x^2)}^{-\frac{1}{2}} \\
        (1 + x^2)y' = & \ (1 + x^2) * x {(1 + x^2)}^{-\frac{1}{2}} \\
        = & \ x {(1 + x^2)}^{\frac{1}{2}} \\
        = & \ xy.
      \end{align*}
    \end{proof}

    \item \(y = ae^x + be^{-x}\) is a solution to \(y'' - y = 0\)
    \begin{proof}
      \begin{align*}
        y' = & \ ae^x - be^{-x} \\
        y'' = & \ ae^x + be^{-x} \\
        y'' - y = & \ ae^x + be^{-x} - (ae^x + be^{-x}) \\
        = & \ 0.
      \end{align*}
    \end{proof}

  \end{enumerate}
  
\end{enumerate}


\pagebreak
\section*{Section 2}

\begin{enumerate}
  \item Determine the order of each differential equation and whether it is linear or non-linear. If it is linear, determine if its is homogenous or non-homogenous.
  \begin{enumerate}
    \item \(y'' - \cos(t)y = e^{t}y'\)
    
    Order: 2, Linear, Homogenous

    \item \({(y')}^3 = 2y\)
    
    Order: 1, Non-Linear

    \item \(e^{y^{(4)}} + y'' - y = y'\)
    
    Order: 4, Non-Linear

    \item \(ty'' + \cos(t) + y = 0\)
    
    Order: 2, Linear, Non-Homogeneous

  \end{enumerate} 
\end{enumerate}

\end{document}